nits

src/c/HWAbstraction.c
@@ -2,28 +2,28 @@
 
 uint32_t uds_len = 32;
 
-HWState_state st = {
-		    (uint8_t *) 1,        /* cdi */
-		    1U,                   /* l0 image header size */
-		    (uint8_t *) 1,        /* l0 image header */
-		    (uint8_t *) 1,        /* l0 image header signature */
-		    1U,                   /* l0 binary size */
-		    (uint8_t *) 1,        /* l0 binary */
-		    (uint8_t *) 1,        /* l0 binary hash */
-		    (uint8_t *) 1 };      /* l0 image authentication key */
-
-void read_uds(uint8_t *uds) {
-  return;
+HWState_state st ()
+{
+  HWState_l0_image_t img = { 1U, (uint8_t *) 1,
+		     (uint8_t *) 1, 1U, (uint8_t *) 1,        
+	(uint8_t *) 1, (uint8_t *) 1 };
+  HWState_state sta = { (uint8_t *) 1, img };
+  return sta;
 }
 
-void platform_zeroize_stack () {
-  return;
+  void read_uds(uint8_t *uds) {
+			       return;
 }
+
+  void platform_zeroize_stack () {
+				  return;
+  }
 
 void disable_uds () {
-  return;
+		     return;
 }
 
 void platform_zeroize (uint32_t len, uint8_t* buf) {
-  return;
+						    return;
 }
+
