src/dice/HWState.fsti
@@ -15,11 +15,7 @@ type mbuffer (a:Type0) (len:nat) =
 val t : Type0
 
 noeq
-type state = {
-  ghost_state : mbuffer (G.erased t) 1;
-
-  cdi : mbuffer byte_sec (v digest_len);
-
+type l0_image_t = {
   l0_image_header_size : signable_len;
   l0_image_header      : mbuffer byte_sec (v l0_image_header_size);
   l0_image_header_sig  : mbuffer byte_sec 64;
@@ -27,12 +23,27 @@ type state = {
   l0_binary            : mbuffer byte_sec (v l0_binary_size);
   l0_binary_hash       : mbuffer byte_sec (v digest_len);
   l0_image_auth_pubkey : b:mbuffer byte_sec 32{
-    B.(all_disjoint [loc_buffer ghost_state;
-                     loc_buffer cdi;
-                     loc_buffer l0_image_header;
+    B.(all_disjoint [loc_buffer l0_image_header;
                      loc_buffer l0_image_header_sig;
                      loc_buffer l0_binary;
                      loc_buffer l0_binary_hash;
                      loc_buffer b ])
+  }
+}
+
+noeq
+type state = {
+  ghost_state : mbuffer (G.erased t) 1;
+
+  cdi : mbuffer byte_sec (v digest_len);
+
+  l0 : img:l0_image_t{
+    B.(all_disjoint [loc_buffer ghost_state;
+                     loc_buffer cdi;
+                     loc_buffer img.l0_image_header;
+                     loc_buffer img.l0_image_header_sig;
+                     loc_buffer img.l0_binary;
+                     loc_buffer img.l0_binary_hash;
+                     loc_buffer img.l0_image_auth_pubkey ])
   }
 }
