src/dice/HWAbstraction.fsti
@@ -21,32 +21,49 @@ val uds_len : hashable_len
 
 val uds_bytes : s:G.erased bytes_sec{Seq.length (G.reveal s) == v uds_len}
 
-val st : state
+val st (_:unit) : state
 
-let st_liveness (h:HS.mem) : Type0 =
+let st_liveness (st:state) (h:HS.mem) : Type0 =
   B.all_live h [
     B.buf st.ghost_state;
     B.buf st.cdi;
-    B.buf st.l0_image_header;
-    B.buf st.l0_image_header_sig;
-    B.buf st.l0_binary;
-    B.buf st.l0_binary_hash;
-    B.buf st.l0_image_auth_pubkey ]
+    B.buf st.l0.l0_image_header;
+    B.buf st.l0.l0_image_header_sig;
+    B.buf st.l0.l0_binary;
+    B.buf st.l0.l0_binary_hash;
+    B.buf st.l0.l0_image_auth_pubkey ]
 
 inline_for_extraction noextract
-let recall_st_liveness ()
+let recall_image_liveness (img:l0_image_t)
   : Stack unit
       (requires fun _ -> True)
       (ensures fun h0 _ h1 ->
         h0 == h1 /\
-        st_liveness h1)
+        B.live h1 img.l0_image_header /\
+        B.live h1 img.l0_image_header_sig /\
+        B.live h1 img.l0_binary /\
+        B.live h1 img.l0_binary_hash /\
+        B.live h1 img.l0_image_auth_pubkey)
+  = B.recall img.l0_image_header;
+    B.recall img.l0_image_header_sig;
+    B.recall img.l0_binary;
+    B.recall img.l0_binary_hash;
+    B.recall img.l0_image_auth_pubkey
+  
+inline_for_extraction noextract
+let recall_st_liveness (st:state)
+  : Stack unit
+      (requires fun _ -> True)
+      (ensures fun h0 _ h1 ->
+        h0 == h1 /\
+        st_liveness st h1)
   = B.recall st.ghost_state;
     B.recall st.cdi;
-    B.recall st.l0_image_header;
-    B.recall st.l0_image_header_sig;
-    B.recall st.l0_binary;
-    B.recall st.l0_binary_hash;
-    B.recall st.l0_image_auth_pubkey
+    B.recall st.l0.l0_image_header;
+    B.recall st.l0.l0_image_header_sig;
+    B.recall st.l0.l0_binary;
+    B.recall st.l0.l0_binary_hash;
+    B.recall st.l0.l0_image_auth_pubkey
 
 val uds_is_enabled (h:HS.mem) : Type0
 
@@ -55,9 +72,9 @@ val stack_is_erased (h:HS.mem) : Type0
 val frame_ghost_state (l:B.loc) (h0 h1:HS.mem)
   : Lemma
       (requires
-        B.(loc_disjoint (loc_buffer st.ghost_state) l) /\
+        B.(loc_disjoint (loc_buffer (st ()).ghost_state) l) /\
         B.(modifies l h0 h1) /\
-        B.live h0 st.ghost_state)
+        B.live h0 (st ()).ghost_state)
       (ensures
         uds_is_enabled h0 == uds_is_enabled h1 /\
         stack_is_erased h0 == stack_is_erased h1)
@@ -78,7 +95,7 @@ val disable_uds (_:unit)
       (ensures fun h0 _ h1 ->
         (~ (uds_is_enabled h1)) /\
         stack_is_erased h0 == stack_is_erased h1 /\
-        B.(modifies (loc_buffer st.ghost_state) h0 h1))
+        B.(modifies (loc_buffer (st ()).ghost_state) h0 h1))
 
 val platform_zeroize_stack (_:unit)
   : Stack unit
@@ -86,7 +103,7 @@ val platform_zeroize_stack (_:unit)
       (ensures fun h0 _ h1 ->
         (~ (uds_is_enabled h1)) /\
         stack_is_erased h1 /\
-        B.(modifies (loc_buffer st.ghost_state) h0 h1))
+        B.(modifies (loc_buffer (st ()).ghost_state) h0 h1))
 
 val platform_zeroize (len:I.size_t) (b:B.lbuffer byte_sec (v len))
   : Stack unit
